8/26/25

1. Simplify the following.  
	a. $$2x^2 -5y +4x +1 +2y -3x$$
		Solution: $$ \boxed{2x^2 +x -3y +1} $$
	b. $$\sqrt{9+16}$$
		Solution: $$\sqrt{25} = \sqrt{5^2} = \sqrt{5}^2 = \boxed5$$
	c. $$\sqrt{4+9+3}$$
		Solution: $$\sqrt{16} = \sqrt{4^2} = \boxed4$$
	d. $$\sqrt{48}$$ 
		Solution: $$\sqrt{3*16} = \sqrt{3}\cdot\sqrt{4^2} = \boxed{4\sqrt{3}}$$ 
	e. $$4 \sqrt{12} - 2 \sqrt{75}$$
		Solution: $$4 \sqrt{12} - 2 \sqrt{75} = 4 \sqrt{4 \cdot 3} - 2 \sqrt{25 \cdot 3}$$$$= 4(2)\sqrt{3} - 2(5)\sqrt{3}$$$$= 8\sqrt{3} - 10\sqrt{3}$$$$=\boxed{-2 \sqrt{3}}$$
	f. $$\frac{h^2+2ah}{h}$$
		Solution: $$\frac{h(h+2a)}{h} = \frac{\cancel{h}(h+2a)}{\cancel{h}} = \boxed{h+2a}$$
	g. $$(x-8)^2$$
		Solution: $$(x-8)(x-8) = \boxed{ x^2 -16x +64 }$$
	h. $$64 - 4(7 + 1)$$
		Solution: $$ 64 - 4(8) = 64 -32 = \boxed{32} $$
	i. $$-15-2^2$$
		Solution: $$-15-4 = \boxed{-19}$$
	j. $$\frac{(3x^4)^2 6xy^{-7}}{3(2x)^3y^2} $$
		Solution: $$= \frac{9x^8 6xy^{-7}}{3(8x^3)y^2} = \frac{\cancelto{3}{9}x^\cancelto{6}{8} \cancelto{3}{6}\cancel{x}y^{-7}}{\cancelto{1}{3}*\cancelto{4}{8}\cancel{x^3}y^2} = \frac{3x^6 3y^{-7}}{4y^2} = \boxed{\frac{9x^6}{4y^9}}$$
	k. $$\frac{5*2-(4-7)^2}{[\frac{1}{2}(3^2 - (2-5))]^2}$$
		Solution: $$= \frac{10 - (-3)^2}{[\frac{1}{2} (9 (-3))]^2} = \frac{10-9}{[\frac{1}{2}(12)]^2} = \frac{1}{(6)^2} = \boxed{\frac{1}{36}}$$
	l. $$(\frac{-8x^3}{y^{-6}})^{2/3} (\frac{-x^{-2/3} y^{3/2}}{y^{-1/3}})^3$$
		Solution: $$\begin{aligned} 
		&= (-8x^3 y^6)^{2/3} (-x^{-2/3} y^{11/6})^3 \\
		&= (4x^2 y^4) (-x^{-2} y^{11/2}) \\
		&= -4x^0 y^{19/2} \\
		&= \boxed{-4y^{19/2}\space \text{or}\space -4y^{9.5}}\\
		\end{aligned}$$

2. Factor the following.  
	a. $$ x^2 -1 $$
		Solution:  [[Difference of Squares]] $$ = x^2 -1^2 = (x+i)(x-i) $$
	b. $$ x^2 +7x +6 $$
		Solution: [[Quadratic Trinomial Formula]] $$ (x+6)(x+1) $$

	c. $$ x^2-4x+3 $$
		Solution: [[Quadratic Trinomial Formula]] $$ (x-3)(x-1) $$
	d. $$ 6x^4 -7x^2 -5 $$
		Solution: [[U Substitution]] and [[Quadratic Trinomial Formula]]$$ u = x^2$$$$ 6u^2 -7u -5 = (6u^2 +3u) +(-10u -5) = 3u(2u +1) -5(2u +1)) $$$$= (3u -5) (2u+1) = (2x^2 +1) (3x^2-5)$$
	e. $$ x^3 -6x^2 -4x +24 $$  
			Solution:  Grouping, factoring out, and then [[Quadratic Trinomial Formula]] $$ = x^2(x -6) -4(x -6) = (x^2 -4) (x -6) = (x-2)(x+2)(x-6) $$
	f. $$ 9x^3 y +6xy^2 $$
		Solution: reverse of [[The Distributive Property]] $$ \to\quad 3xy(3x^2+2y)$$
	g. $$ x^4 -16 $$
		Solution: Recursive [[Difference of Squares]]$$ = (x^2+4)(x^2-4) = (x^2+4)(x-2)(x+2) $$
	h. $$ 4x^3 -2x^2 +6x -3 $$
		Solution: Grouping and factoring out $$ (4x^3 -2x^2) (+6x-3) = 2x^2(2x-1) 3(2x-1) = (2x^2+3)(2x-1) $$
	i. $$ (6x-5)^3 (2) (x^2 +4) (2x) +(x^2+4) (3) (6x-5)^2 (6) $$
		Solution: $$ (x^2+4)^2(6x-5)^5 (2)(2x)(3)(6) = (x^2+4)^2(6x-5)^2 (72x)$$

3. Solve the following.  
	a. $$ 4(x -1) = 3-(2 +x) $$
		Solution: $$ \to 4x-4 = 3+-2-x \to 5x = 5 \to x = 1 $$
	b. $$ 3x +2(x -10) = 5(x-4) $$
		Solution: $$ 3x+2x-20 = 5x-20 \to 5x -20 = 5x-20 \to 0 = 0 \to \text{true for all x}$$
	c. $$ x^2 -x = 6 $$
		Solution: [[Quadratic Trinomial Formula]] $$ x^2-x-6 = 0 \to (x^2 -3x)+(2x-6) \to x(x-3) +2(x-3) = 0 \to (x-3)(x+2)=0 $$ $$ \to (3, -2)$$
	d. $$ 2x^2 -4x+3 = 0 $$
		Solution: [[Quadratic Formula]] $$ \begin{aligned}
		x_{1,2} =&\space {-(-4)\pm\sqrt{(-4)^2-4\cdot2 \cdot 3} \over 2 \cdot 2}\\\\
		
		x_{1,2} =&\space {4\pm\sqrt{-8}\over4} \quad\to\quad {4\pm2\sqrt{2}i\over4}\\\\
		
		x_1 =&\space1+i{\sqrt{2}\over2}\quad x_2 = 1-i{\sqrt2\over2}
		\end{aligned}$$2
	e. $$ x^3 +84x =19x^2 $$
		Solution: $$ \begin{aligned}
		&x(x^2-19x+84) = 0\\
		&x(x-12)(x-7) \\
		&\boxed{x = 0, 12, 7}
		
		\end{aligned}$$
	f. $$ -10x \geq 30 $$
		 Solution: $$\frac{\cancel{-10}x}{\cancel{-10}} \geq \frac{30}{-10} \to x \leq-3$$ 
	g. $$ -2 \leq 3r-7 \lt 2$$
		Solution: `Split the inequality apart`$$ -2 \leq 3r-7 \space \text{and} \space 3r-7 \lt 2$$ `Solve individually` $$
		 -2 \leq 3r -7 
		\to 5 \leq 3r 
		\to \frac{5}{3} \leq r
		\to r \geq \frac{5}{3}
		$$ $$ 
		3r -7 < 2
		\to 3r < 9
		\to r < 3 
		$$ `All together:` $$ 3/5 \leq r < 3 $$
	h. $$ 0 \lt \frac{1}{3} (4 -x) -10 \leq 16$$
		Solution: `Split apart` $$\begin{aligned}
		&0 < \frac{1}{3}(4-x) -10 \\\\
		&\to \quad 10 < \frac{1}{3}(4-x)\\\\
		&\to \quad 30 < 4-x\\
		&\to \quad 26 < -x\\
		&\to \quad -26 > x\\
		&\to \quad x < -26
		\end{aligned}$$ $$ \begin{aligned}
		&\frac{1}{3}(4-x) -10\leq 16 \\\\
		&\to \frac{1}{3}(4-x) \leq 26 \\\\
		&\to 4 -x \leq 78 \\
		&\to -x \leq 74 \\
		&\to x \geq -74 \\
		\end{aligned} $$
		`Recombine:` $$ \boxed{-74 \leq x < -26} $$
	i. $$ \frac{x -2}{x +4} \leq 0 $$
		Solution: `Identify intervals` 
		$f(2) = 0$
		$f(-4) = undefined$ (vertical asymptote) $$-4 < x \leq 2$$
	j. $$ x^2 +2x +1 \gt 0$$
		Solution: [[Parabolas]] `Factor the parabola`  $$ (x+1)^2 > 0 $$ This will only be 0 when $x+1 = 0$, or $x=-1$, which means $$(-\infty, -1) \cup (-1, \infty)  $$ 
	k. $$|-5x+10| \lt 30 $$
		Solution: $$\to\quad -30 <-5x+10 < 30 \quad \to\quad -40 < -5x < 20$$ $$ 8 > x > -4 $$
	l. $$ 2 \log_{3}(x +1) -5 = -1 $$
		Solution: $$ \to \quad 2log_3(x+1) = 4 \quad \to\quad log_3(x+1) = 2 \quad \to \quad log_3(x+1) = log_3(9)$$ $$ \to x+1=9 \quad \to \quad x = 8 $$ 
	m. $$ 3 \times 0.25^x +5 = 11 $$
		Solution: $$\to \quad 3\cdot 0.25^x = 6 \quad \to \quad 0.25^x = 2$$ $$\to \quad \ln 0.25^x = \ln2 \quad \to \quad x\ln0.25 = \ln2 \quad \to \quad x=\frac{\ln2}{\ln0.25} \to \frac{\ln2}{\ln{1\over4}}$$ $$\to \frac{\ln2}{\ln2^{-2}} \to \frac{\ln2}{-2\ln2} \to -{1\over2}$$
 
4. Find the domain of the following functions. Write your answer in interval notation.  
	a. $$ f(x) = \frac{x}{ \sqrt{x+3}} $$
		Solution:
		[[Rules of Roots|Root]] does not calculate below 0 in real numbers 
		$$ 
		x +3 \geq 0 = x \geq -3
		$$  $$ =(-3, \infty )$$
	
	b. $$ g(x) = \ln(5-2x)$$
		Solution:
		[[Rules of Logarithms|Logarithm]]'s domain is $\gt 0$ $$ 5 -2x \gt 0 \quad \to \quad -2x \gt 5 \quad \to \quad x < {5 \over 2} \quad \to (-\infty, {5\over2}) $$ 
	c. $$ h(x) = e^{7x+1} + 8x^2 $$
		Solution: **No constraints** $$(-\infty, \infty)$$

5. Rationalize the numerator and simplify.  
	a. $$ \frac{\sqrt{x}-\sqrt{y}}{x^2-y^2}$$
		Solution: [[Rules of Roots|Root]] $$ 
		\begin{aligned}
		\to& \quad \frac{(\sqrt{x} - \sqrt{y} ) \cdot (\sqrt{x}+\sqrt{y})} {(x^2 -y^2) \cdot (\sqrt{x}+\sqrt{y})} \\\\
		
		\to& \quad \frac{x-y}{(x-y)(x+y)(\sqrt{x}+\sqrt{y})} \\\\
		
		\to& \quad \boxed{\frac{1}{(x+y)(\sqrt{x}+\sqrt{y})}}
		\end{aligned}
		$$ 
	b.$$ \frac{\sqrt{2 (x+h) +1} - \sqrt{2x+1}} {h} $$
		Solution: $$\begin{aligned}
		&\text{Multiply by conjugate}\\
		\to& \quad  \frac
		{(\sqrt{2 (x+h) +1} - \sqrt{2x+1}\space) \cdot(\sqrt{2 (x+h) +1} + \sqrt{2x+1})} 
		{h\cdot (\sqrt{2 (x+h) +1} + \sqrt{2x+1})} \\\\
		
		\to& \quad \frac{(2x+2h+1) - (2x+1)}{h\cdot (\sqrt{2 (x+h) +1} + \sqrt{2x+1})} \\\\
		
		\to& \quad \frac{2}{\sqrt{2 (x+h) +1} + \sqrt{2x+1}}
		\end{aligned}
		$$

6. Difference quotients
	a. What is the difference quotient? What does it represent? [[Difference Quotient]] $$\frac{f(x+h)-f(x)}{h}$$
	b. Given that $f(x) = x^2 -3x +9$. Find and simplify the difference quotient.
		Solution: $$ \begin{aligned}
		\to& \quad \frac{[(x+h)^2-3(x+h) +9] -(x^2-3x+9)}{h} \\\\
		\to& \quad \frac{[x^2+2xh+h^2 -3x -3h +9]-(x^2-3x+9)}{h} \\\\
		\to& \quad \frac{x^2+2xh+h^2-3x-3h+9-x^2+3x-9}{h} \\\\
		\to& \quad \frac{h^2 +2xh -3h }{h}
		\quad \to \quad \frac{\cancel{h}(h+2x-3)}{\cancel{h}} 
			\quad \to \quad \boxed{{2x+h-3}}
		\end{aligned}
		$$
	c. Given that $g(x) = \frac{5}{x+1}$. Find and simplify the difference quotient.
		Solution: $$\begin{aligned}
		\to& \quad \frac{(\frac{5}{x+h+1})-(\frac{5}{x+1})}{h} \\\\
		\to& \quad \frac{\frac{5(x+1)}{(x+h+1)(x+1)} - \frac{5(x+h+1)}{(x+h+1)(x+1)}} {h} \\\\
		\to& \quad \frac{ \frac{-5h }{(x+h+1)(x+1)}} {h\over1} \to \frac{-5h}{(x+h+1)(x+1)h} \\\\
		\to& \quad \frac{-5\cancel{h}}{\cancel{h}(x+h+1)(x+1)} \to \boxed{\frac{-5}{(x+h+1)(x+1)}}
		\end{aligned}$$
	d. Given that $h(x) = \sqrt{x-3}$. Find and simplify the difference quotient.
		Solution: $$\begin{aligned}
		\to& \quad \frac{(\sqrt{(x+h)-3}\space) - (\sqrt{x-3}\space)}{h} \\\\
		
		\to& \quad \frac{[(\sqrt{(x+h)-3}\space) - (\sqrt{x-3}\space)] \cdot[(\sqrt{(x+h)-3}\space) + (\sqrt{x-3}\space)]} {h \cdot [(\sqrt{(x+h)-3}\space) + (\sqrt{x-3}\space)]} \\\\
		
		\to& \quad \frac{x+h-3 -x +3}{h \cdot (\sqrt{(x+h)-3}+ \sqrt{x-3}\space)} \\\\
		
		\to& \quad \frac{\cancel{h}}{\cancel{h} \cdot (\sqrt{(x+h)-3}+ \sqrt{x-3}\space)} \\\\
		
		\to& \quad \boxed{ \frac{1}{\sqrt{x+h-3}+\sqrt{x-3}} }
		\end{aligned}
		$$

7. Evaluate the function as indicated and simplify  
	a. $f(x) = \frac{3x}{x-5}$
		1. $f(-1)$ $$ \frac{3(-1)}{(-1)-5} \to \frac{-3}{-6}\to \boxed{\frac{1}{2}}$$
		2. $f(\frac{1}{2})$ $$ \frac{3(\frac{1}{2})} {(\frac{1}{2})-5} \to \frac{3\cdot1}{1-10} \to \frac{3}{-9}\to \boxed{-\frac{1}{3}} $$
		3. $f(x+1)$ $$ \frac{3(x+1)}{(x+1)-5} \to \boxed{\frac{3x+3}{x-4}} $$
		
	b. $f(x) = \begin{cases} x+8 & \text{if } x \lt 0 \\ 10 -2x & \text{if } x \geq 0 \end{cases}$
		(i) $f(4)$ $$ 10-2(4) \to 10-8 \to \boxed{2}$$
		(ii) $f(0)$ $$10 - 2(0) \to \boxed{10}$$
		(iii) $f(6) - f(-2)$ $$( 10 -2(6) ) - ( (-2) +8) \to (-2)-6=\boxed{-8}$$

8. Find and simplify $(f \circ g)(x) = f(g(x))$ for each of the following:
	a. $f(x) = x^2+3$, $f(g) = 4x -1$ $$ (4x-1)^2+3 \to 16x^2-8x+1+3 \to \boxed{16x^2-8x+4} $$
	b. $f(x)= 6x-3$, $g(x)=\frac{x+3}{6}$ $$6(\frac{x+3}{6})-3 \quad\to\quad  \frac{\cancel6 (x+3)}{\cancel6}-3 \quad\to\quad (x+3)-3 \quad\to\quad  \boxed x$$
	c. $f(x)= 5x-2$, $g(x)=-x^2 +4x -1$ $$5(-x^2+4x-1)-2 \quad\to\quad \boxed{-5x^2 +20x -7} $$

9. $h(x)$ is a composition of two simpler functions $f$ and $g$ where $h(x)=f(g(x))$. Identify $f(x)$ and $g(x)$
	a. $h(x)=(2x-7)^4$ $$ \begin{aligned}
	&f(x)=x^4 \\
	&g(x)=2x-7
	\end{aligned}
	$$
	b. $h(x)=\sin(x^2+1)$ $$ \begin{aligned}
	&f(x)=\sin x \\
	&g(x) = x^2+1
	\end{aligned}
	$$
	c. $h(x)=\cos^2x$ $$ \begin{aligned}
	&f(x) = x^2 \\
	&g(x) = \cos x
	\end{aligned} $$

10. How many radians is 225Â°?  
	Solution: [[Converting Degrees to Radians]] $$ {225\cancel\degree \pi \over 180\cancel\degree} \quad\to\quad \boxed{\frac{5 \pi}{4}}$$


11. Find the exact value of $\tan(\frac{5\pi}{3})$ [[Tangent|Tan]] 
	Solution: $$ \begin{gather}
	\tan \theta = \frac{\sin \theta}{\cos \theta}\\\\
	
	\to\quad \frac{\sin({5 \pi \over 3})}{ \cos ({5 \pi \over 3})}
	
	\quad\to\quad &\frac{-\frac{\sqrt3}{2}}{1\over2}
	
	\quad\to\quad -\frac{\cancel2 \sqrt{3}} {\cancel2} \quad= \boxed{-\sqrt{3}}
	\end{gather} $$

12. Find all solutions to $cos^{-1}(\frac{-1}{\sqrt{2}})$ on the interval $0 \leq \theta \lt 2\pi$ 
    Solution: $$\begin{aligned}
    \to\quad &\arccos({-1\over \sqrt{2}}) \quad \text{(Q2, Q3)} \\\\
    
    \to\quad &\pi \pm \frac{\pi}{4} \space\text{or}\space \frac{3\pi}{4}\space\text{and}\space \frac{5\pi}{4} 
    \end{aligned}$$ 

13. On a certain right triangle $\sin\theta = \frac{x}{2}$. Find the values of the 5 other trig expressions.
    Solution: [[Sine|Sin]] $$\begin{aligned}   
    \text{Opposite: }& x \\
    \text{Hypoteneuse: }& 2 \\
    \text{Adjacent: }& \sqrt{4-x^2}\\
    \end{aligned}$$ $$ \begin{aligned}
    \sin\theta &= \frac{x}{2} \\\\
    
    \cos\theta &= \frac{\sqrt{4-x^2}}{2} \\\\
    
    \tan\theta &= \frac{\frac{x}{2}}{\frac{\sqrt{4-x^2}}{2}} \to \frac{x}{\sqrt{4-x^2}} \\\\
    
    \sec\theta &= \frac{2}{\sqrt{4-x^2}}\\\\
    
    \csc\theta &= \frac{2}{x} \\\\
    
    \cot\theta &= \frac{\sqrt{4-x^2}}{x} \to
    \end{aligned}$$

14. At what point(s) does the parabola $y=x^2-3x-10$ intersect the line $y=x+2$ ?
    Solution: [[Parabolas]] and [[Quadratic Trinomial Formula]]$$ \begin{aligned}
    &\text{System of equations}\\
    y &= x^2-3x-10\\
    y &= x+2 \\\\
    
    &\text{Substitute, then factor}\\
    x+2 &=x^2-3x-10 \\
    0 &= x^2-4x-12\\
    &\to (x+2)(x-6) \to x=-2,6 \\\\
    &\text{Plug back in x values to find y}\\  
    y &= -2+2 =0 \quad\to\boxed{(-2, 0)} \\
    y &= 6+2 = 8 \;\;\;\quad\to\boxed{(6, 8)}
    \end{aligned}$$

15. Find the equation of the line that has the point $(3,1)$ and is parallel to the line $y=\frac{1}{2}x -13$ .
	Solution: [[Point Slope Form]] $$\begin{aligned} 
	\to\quad& y-1 = \frac{1}{2}(x-3) \\\\
	\to\quad& y = \frac{1}{2}x - \frac{3}{2}+1 \\\\
	\to\quad& \boxed{y = \frac{1}{2}x - \frac{1}{2}}
 \end{aligned}$$